verified-ocaml/instruct-verification/theories/test_iv.v
@@ -6,7 +6,7 @@ Require Import PUSH_RETADDR_correct.
 (* The types must match: use InstructSpec's push_retaddr_step_pre *)
 Lemma test : forall ret_addr,
     handler_correct (Interpret.handle_PUSH_RETADDR ret_addr) f_instr_PUSH_RETADDR
-      (fun _ m s ard => InstructSpec.push_retaddr_step_pre ret_addr m s ard)
+      (InstructSpec.push_retaddr_step_pre ret_addr)
       (fun _ _ => False) (fun _ => False) (fun _ _ _ => False).
 Proof.
   exact verify_PUSH_RETADDR_correct.
